src/Util/Tactics.v
@@ -2,3 +2,20 @@ Ltac destruct_hypos := repeat (match goal with
   | H : exists a, _ |- _ => destruct H
   | H : ?x /\ ?y |- _ => destruct H
   end).
+
+
+Ltac destruct_if :=
+  match goal with
+    | |- context[if ?X then _ else _] => destruct X eqn:H_eqb
+  end.
+
+Ltac destruct_match :=
+   match goal with
+   | |- context[match ?X with | _ => _ end] => destruct X eqn:H_match
+   end.
+
+Ltac destruct_match_hypo :=
+   match goal with
+   | H : context[match ?X with | _ => _ end] |- _ => destruct X
+   end.
+
